stupid attempt at writing a predicate as in the solution sketch

io/Hyperproperties.fst
@@ -100,10 +100,23 @@ val ni :
 //   ctx == dm_giio_bind (inst_io_cmds pi cmd arg) cont
 //   ctx == dm_giio_bind (eff_rc x) (fun eff_rc' -> dm_giio_bind cont1 (fun y -> dm_giio_bind (eff_rc' y) cont2)
 // with that, one can do induction on the ctx to prove the non-interference
-
 // there is no axiom/law for erased
 // pi is Tot, it does not matter that it is erased
 // 
+
+assume val __reify_IIOwp (#a:Type) (#wp:Hist.hist a) (#fl:tflag) ($f:unit -> IIOwp a fl wp) : Tot (dm_giio a fl wp)
+  
+let rec only_pi_and_rc (pi:monitorable_prop) (eff_rc:eff_rc_typ AllActions #'a #'b 'rc) (m:dm_giio int AllActions trivial_hist) : GTot Type0 (decreases m) =
+  (exists r. m == Return r) \/
+  (exists cmd arg (cont:io_resm cmd arg -> dm_giio int AllActions trivial_hist).
+    (m == dm_giio_bind _ int _ _ _ _ (__reify_IIOwp (fun () -> inst_io_cmds pi cmd arg <: IIOwp (io_resm cmd arg) AllActions trivial_hist)) cont) /\
+    (forall r. only_pi_and_rc pi eff_rc (cont r))) \/
+  (exists x (cont1:dm_giio 'b AllActions trivial_hist) (cont2: _ -> dm_giio int AllActions trivial_hist). 
+    only_pi_and_rc pi eff_rc cont1 /\
+    (forall r. only_pi_and_rc pi eff_rc (cont2 r)) /\
+    m == dm_giio_bind _ int AllActions AllActions trivial_hist (fun _ -> trivial_hist) (__reify_IIOwp (fun () -> eff_rc x)) 
+                      (fun (| _, eff_rc' |) -> dm_giio_bind _ int AllActions AllActions trivial_hist (fun _ -> trivial_hist) cont1 
+                                                         (fun y -> dm_giio_bind _ int _ _ _ _ (__reify_IIOwp (fun () -> (eff_rc' y))) cont2)))
 
 let ni pi rc ctx = admit ()
 
